---
tags:
  - m
  - 3te_Klasse
---
3.28a)
```math
||{"id":1609097473726}||

f(x)=2x²+2x+1
f'(x)=4x¹+2
```
c)
```math
||{"id":50981288364}||

f(x)=\frac{3}{x²}-\frac{4}{x}=3x^{-2}-4x^{-1}
f'(x)=-6x^{-3}+4x^{-2}=-\frac{6}{x³}+\frac{4}{x²}
```
f)
```math
||{"id":249053329159}||

f(x)=\frac{x²+1}{2x}=\frac{x²}{2x}+\frac{1}{2x}=\frac{x}{2}+\frac{x^{-1}}{2}
f'(x)=\frac{1}{2}-\frac{1x^{-2}}{2}=-\frac{1}{2x²}+\frac{1}{2}
```
3.26)
a)
```math
||{"id":1454345359785}||

f(x)=2x²
f'(x)=2*2x^{2-1}=4x
```
b)
```math
||{"id":877527017994}||

f(x)=\frac{x}{2}
f'(x)=\frac{1*x^{1-1}}{2}=\frac{1*x^{0}}{2}=\frac{1}{2}
```

c)
```math
||{"id":970221368795}||

f(x)=2x^{-1}
f'(x)=-1*2x^{-1-1}=-1*2x^{-2}=-2x^{-2}=\frac{.2}{x²}
```
d)
```math
||{"id":757498232671}||

f(x)=\frac{1}{3x}=\frac{x^{-1}}{3}
f'(x)=\frac{-1x^{-2}}{3}=-\frac{1}{3x²}
```
e)
```math
||{"id":1352343433582}||

f(x)=\frac{1}{x²}=x^{-2}
f'(x)=-2x^{-3
```

<div tabindex='-1'contenteditable='false' class='livePrevPlus'></div>
