2.21)
a)
```math
||{"id":1076189461997}||

y=\frac{1}{x}
\lim_{ x \to \infty } \frac{1}{x}=0
\lim_{ x \to -\infty } \frac{1}{x}=0
```

b)
```math
||{"id":1368027710396}||

y=\frac{1}{x-2}
\lim_{ x \to \infty } \frac{1}{x-2}=0
\lim_{ x \to -\infty } \frac{1}{x-2}=0
```

g)
```math
||{"id":582868932643}||

y=\frac{6x²-3}{2x²+x+1}
\lim_{ x \to \infty } \frac{6x²-3}{2x²+x+1}=3
\lim_{ x \to -\infty } \frac{6x²-3}{2x²+x+1}=3
```

2.22
a)
```math
||{"id":1017300411637}||

y=\frac{x²}{x-1}
(x²):(x-1)=x
(x²+x)
x
```

d)
```math
||{"id":1581286767132}||

y=\frac{x^2-2}{2(x-2)}
y=\frac{x^2-2}{2x-4}
(x²-2):(2x-4)=
2x
```

2.23
a)
```math
||{"id":702177955070}||

\lim_{ x \to \infty } \frac{\sqrt{ x²+1 }}{x}=1
```

b)
```math
||{"id":458273688883}||

\lim_{ x \to \infty } \frac{3+2x}{1+2x}=1
```

2.25
```math
||{"id":166064668530}||


```
